add surface syntax

Applib/Surface/Object.lean
@@ -4,14 +4,26 @@ namespace Applib
 
 open AVM
 
-class IsObject (S : Type) where
-  label : Ecosystem.Label
-  classId : label.ClassId
+class IsObjectOf {lab : Ecosystem.Label} (classId : lab.ClassId) (S : Type) where
   toObject : S → ObjectData classId
   fromObject : ObjectData classId → S
   left_inverse : fromObject ∘ toObject = id := by rfl
 
-lemma IsObject.left_inverse' {S : Type} [i : IsObject S] (s : S)
+class IsObject (S : Type) where
+  label : Ecosystem.Label
+  classId : label.ClassId
+  isObjectOf : IsObjectOf classId S
+
+abbrev IsObject.toObject {S} (i : IsObject S) : S → ObjectData i.classId := i.isObjectOf.toObject
+
+abbrev IsObject.fromObject {S} (i : IsObject S) : ObjectData i.classId → S := i.isObjectOf.fromObject
+
+lemma IsObjectOf.left_inverse'
+  {lab : Ecosystem.Label}
+  {classId : lab.ClassId}
+  {S : Type}
+  [i : IsObjectOf classId S]
+  (s : S)
   : i.fromObject (i.toObject s) = s := by
   rw [← Function.comp_apply (f := fromObject) (g := toObject)]
   rw [i.left_inverse]
