Applib/Surface/Reference.lean
@@ -1,4 +1,5 @@
 import AVM
+import Applib.Surface.Object
 
 namespace Applib
 
@@ -10,3 +11,17 @@ structure Reference (C : Type) where
 
 instance Reference.hasTypeRep {C : Type} [TypeRep C] : TypeRep (Reference C) where
   rep := Rep.composite "Reference" [TypeRep.rep C]
+
+-- TODO better name?
+structure ObjectReference {lab : Ecosystem.Label} (classId : lab.ClassId) : Type 1 where
+  {type : Type}
+  ref : Reference type
+  [isObjectOf : IsObjectOf classId type]
+
+end Applib
+
+abbrev AVM.Ecosystem.Label.MultiMethodId.SelvesReferences
+  {lab : Ecosystem.Label}
+  (multiId : lab.MultiMethodId)
+  : Type 1
+  := Ecosystem.Label.MultiMethodId.Selves' multiId Applib.ObjectReference
